stuff

Untyped.lean
@@ -9,34 +9,128 @@ namespace Term
 
 protected def repr : Term → String
   | var x => x.repr
-  | abs M => "(λ " ++ Term.repr M ++ ")"
-  | app M N => "(" ++ Term.repr M ++ " " ++ Term.repr N ++ ")"
+  | abs M => "(λ " ++ M.repr ++ ")"
+  | app M N => "(" ++ M.repr ++ " " ++ N.repr ++ ")"
 
 instance instRepr : Repr Term where
   reprPrec M _ := M.repr
 
 def shift' (n k : Nat) : Term → Term
-  | var x => if n ≤ x then var (x + k) else var x
-  | abs M => abs (shift' (n + 1) k M)
+  | var x => if x ≥ n then var (x + k) else var x
+  | abs M => abs (shift' n.succ k M)
   | app M N => app (shift' n k M) (shift' n k N)
 
 def shift : Nat → Term → Term :=
   shift' 0
 
-def subst' (n : Nat) (N : Term) : Term → Term
-  | var x => sorry
-  | abs M => sorry
-  | app M N => sorry
+theorem shift_zero' : ∀ {M}, shift' n 0 M = M
+  | var x => (if h : x ≥ n then if_pos h ▸ rfl else if_neg h ▸ rfl : (if x ≥ n then var x else var x) = var x)
+  | abs _ => congrArg abs shift_zero'
+  | app _ _ => (congr (congrArg app shift_zero') shift_zero' : app _ _ = app _ _)
+
+theorem shift_zero : shift 0 M = M :=
+  shift_zero'
+
+def subst' (n : Nat) (N' : Term) : Term → Term
+  | var x => if x = n then shift n N' else if x > n then var x.pred else var x
+  | abs M => abs (subst' n.succ N' M)
+  | app M N => app (subst' n N' M) (subst' n N' N)
 
 def subst : Term → Term → Term :=
   flip <| subst' 0
 
-#eval abs <| abs <| var 1
-#eval abs <| abs <| abs <| app (app (var 2) (var 0)) (app (var 1) (var 0))
+inductive βred : Term → Term → Prop
+  | β : βred (app (abs M) N) (subst M N)
+  | app₁ : βred M M' → βred (app M N) (app M' N)
+  | app₂ : βred N N' → βred (app M N) (app M N')
+  | ξ : βred M M' → βred (abs M) (abs M')
+
+inductive βred_t : Term → Term → Prop
+  | refl : βred_t M M
+  | trans : βred_t M N → βred_t N O → βred_t M O
+  | β : βred M N → βred_t M N
+
+inductive βeq : Term → Term → Prop
+  | symm : βeq M N → βeq N M
+  | trans : βeq M N → βeq N O → βeq M O
+  | β : βred_t M N → βeq M N
+
+infix:50 " →ᵦ " => βred
+infix:50 " ↠ᵦ " => βred_t
+infix:50 " =ᵦ " => βeq
+
+def Y := abs <| app (abs <| app (var 1) (app (var 0) (var 0))) (abs <| app (var 1) (app (var 0) (var 0)))
+
+def Θ :=
+  let A := abs <| abs <| app (var 0) (app (app (var 1) (var 1)) (var 0))
+  app A A
+
+def βred.symm : βred M N → βeq N M :=
+  βeq.symm ∘ βeq.β ∘ βred_t.β
+
+def βred.trans (h₁ : βred M N) (h₂ : βred N O) : βred_t M O :=
+  (βred_t.β h₁).trans (βred_t.β h₂)
+
+example : app Θ F ↠ᵦ app F (app Θ F) :=
+  βred.β.app₁.trans <| cast
+    (shift_zero ▸ rfl : (_ →ᵦ app (shift 0 F) (app Θ (shift 0 F))) = (_ →ᵦ _))
+    (βred.β : app (abs (app (var 0) (app Θ (var 0)))) F →ᵦ _)
+
+example : app Y F =ᵦ app F (app Y F) :=
+  (βeq.β <| (βred_t.β βred.β).trans <| βred_t.β (βred.β : app (abs <| app (shift 1 F) (app (var 0) (var 0))) (abs <| app (shift 1 F) (app (var 0) (var 0))) →ᵦ _) : app Y F =ᵦ app F (app (abs <| app (shift 1 F) (app (var 0) (var 0))) (abs <| app (shift 1 F) (app (var 0) (var 0))))).trans
+  (βred.β.app₂ : app F (app Y F) →ᵦ app F (app (abs <| app (shift 1 F) (app (var 0) (var 0))) (abs <| app (shift 1 F) (app (var 0) (var 0))))).symm
+
+section
+
+instance : OfNat Term n where
+  ofNat := var n
+
+instance : CoeFun Term λ _ => Term → Term where
+  coe := app
+
+prefix:50 "λ. " => abs
+
+def foo : Term := 2
+def bar : Term := 3
+#eval λ.λ.1
+#eval λ.λ.λ.var 2 0 (var 1 0)
+
+end
+
+def beta : Term → Term
+  | var x => var x
+  | abs M => abs (beta M)
+  | app (abs M) N => subst (beta M) (beta N)
+  | app M N => app (beta M) (beta N)
+
+def beta_normal : Term → Prop :=
+  λ t => beta t = t
+
+def dec (n : Nat) : Term → Option Term
+  | var x => if x = n then none else if x > n then var x.pred else var x
+  | abs M => abs <$> dec n.succ M
+  | app M N => app <$> dec n M <*> dec n N
+
+def eta : Term → Term
+  | var x => var x
+  | abs (app M (var 0)) => let M' := eta M; (dec 0 M').getD <| abs (app (eta M) (var 0))
+  | abs M => abs (eta M)
+  | app M N => app (eta M) (eta N)
+
+def eta_normal : Term → Prop :=
+  λ t => eta t = t
+
+def K := abs <| abs <| var 1
+def S := abs <| abs <| abs <| app (app (var 2) (var 0)) (app (var 1) (var 0))
+def I := app (app S K) K
  
-def ex := app (abs <| abs <| app (app (var 3) (var 1)) <| abs <| app (var 0) <| var 2) <| abs <| app (var 4) <| var 0
+def ex := app (abs <| abs <| app (app (var 3) (var 1)) (abs <| app (var 0) (var 2))) (abs <| app (var 4) (var 0))
 #eval ex
 #eval shift 100 ex
 
+#eval beta ex
+--                  (λ ((2 (λ (5 0))) (λ (0 (λ (6 0))))))
 
--- (λ (3 (λ (6 1))) (λ (1 (λ (7 1)))))
+def ω := abs (app (app (var 0) (var 0)) (var 0))
+#eval app (abs <| var 1) (app ω ω)
+#eval beta <| app (abs <| var 1) (app ω ω)
